mixfix/theorems/MixfixRepairReorder.v
@@ -1,0 +1,71 @@
+From disamb Require Export MixfixRepair.
+From disamb Require Export MixfixReorder.
+From disamb Require Import MixfixReorderTheorems.
+From disamb Require Import MyUtils.
+
+Section MixfixRepairReorder.
+
+Context {T : Type}.
+Implicit Types (t : parse_tree T) (ts : parse_forest T) (p : production T) (X : symbol T)
+  (g : mixfixgrammar T) (Xs : list (symbol T)) (b : bool).
+
+Lemma repair_cl_reorder g Q p t1 ts t' b :
+  wft g E t1 →
+  repair_cl Q p t1 ts = (t', b) → reorder_tree (node p (cons_forest t1 ts)) t'.
+Proof.
+  intro Hwf. revert t' ts b. induction Hwf using well_formed_parse_tree_forest_rec
+    with (P0 := fun p1 t1s Hwfts => ∀ ts ts' b, (b = true ∨ p CL p1 ∠ Q) →
+                            repair_cl_forest Q p t1s ts = (ts', b) →
+                            reorder_tree (node p (cons_forest (node p1 t1s) ts)) (node p1 ts'));
+    intros.
+  - simpl in *. inv H. apply rtc_refl.
+  - simpl in *. destruct (repair_cl_forest Q p ts ts0) eqn:E.
+    destruct (decide (b0 = true ∨ p CL p0 ∠ Q)).
+    + inv H.
+      eapply IHHwf; eauto.
+    + inv H. apply rtc_refl.
+  - simpl in *. exfalso.
+    destruct H.
+    + subst. inv H0.
+    + destruct Q.
+      apply left_pattern_well_formed in H.
+      eapply left_reorderable_nil_false. eassumption.
+  - destruct ts.
+    + destruct (repair_cl Q p t ts0) eqn:F. inv H0.
+      inv w.
+      inv Hwf.
+      * exfalso.
+        simpl in F. inv F.
+        destruct H; try inv H.
+        destruct Q.
+        apply left_pattern_well_formed in H.
+        eapply left_reorder_terminal_false. eassumption.
+      * eapply rtc_l.
+        **repeat constructor.
+        **apply IHHwf in F.
+          apply reorder_forest_reorder_tree.
+          apply reorder_head_tree_reorder_forest.
+          assumption.
+    + destruct (repair_cl_forest Q p (cons_forest p0 ts) ts0) eqn:F. inv H0.
+      simpl in *.
+
+
+Lemma rcl_reorder Q t :
+  reorder_tree t (rcl Q t).
+Proof.
+  induction t.
+  - simpl. apply rtc_refl.
+  - simpl. destruct p0.
+    + apply rtc_refl.
+    + destruct (repair_cl Q p p0 p1) eqn:E.
+
+
+Theorem repair_reorder Q t :
+  reorder_tree t (repair Q t).
+Proof.
+  induction t using parse_tree_forest_rec
+    with (P0 := fun ts => reorder_forest ts (repair_forest Q ts)).
+  - simpl. apply rtc_refl.
+  - cbn [repair]. destruct (repair_forest Q p0) eqn:E.
+    + simpl. apply reorder_forest_reorder_tree. assumption.
+    + 
